src/named/Rule.v
@@ -9,6 +9,7 @@ From Utils Require Import Utils.
 From Named Require Import Term.
 (*TODO: why does this generate warnings?*)
 Import Term.Notations.
+Import SumboolNotations.
 
 Inductive rule : Set :=
 | sort_rule :  ctx -> list string (*explicit args*) -> rule
@@ -290,3 +291,35 @@ Proof.
   unfold ws_lang; intuition.
 Qed.
 #[export] Hint Resolve ws_lang_all_ws_rule : term.
+
+
+Definition rule_eq_dec (r1 r2 : rule) : {r1 = r2} + {~ r1 = r2}.
+  refine(match r1, r2 with
+         | sort_rule c args, sort_rule c' args' =>
+           SB! (ctx_eq_dec c c') SB& (list_eq_dec string_dec args args')
+         | term_rule c args t, term_rule c' args' t' =>
+           SB! (ctx_eq_dec c c') SB&
+           (list_eq_dec string_dec args args') SB&
+           (sort_eq_dec t t')
+         | sort_eq_rule c t1 t2, sort_eq_rule c' t1' t2' =>
+           SB! (ctx_eq_dec c c') SB&
+           (sort_eq_dec t1 t1') SB&
+           (sort_eq_dec t2 t2')
+         | term_eq_rule c e1 e2 t, term_eq_rule c' e1' e2' t' =>
+           SB! (ctx_eq_dec c c') SB&
+           (term_eq_dec e1 e1') SB&
+           (term_eq_dec e2 e2') SB&
+           (sort_eq_dec t t')
+         | _,_ => _
+         end); basic_term_crush.
+Defined.
+
+Definition compute_incl_lang (l1 l2 : lang) :=
+  if incl_dec (pair_eq_dec string_dec rule_eq_dec) l1 l2 then true else false.
+
+Lemma use_compute_incl_lang (l1 l2 : lang)
+  : compute_incl_lang l1 l2 = true -> incl l1 l2.
+Proof.
+  unfold compute_incl_lang.
+  destruct (incl_dec _ l1 l2); easy.
+Qed.
