src/named/SimpleVCPS.v
@@ -15,43 +15,43 @@ Require Coq.derive.Derive.
 
 
 Definition block_subst_def : lang :=
-  [[l
+  {[l
       [s| "G" : #"env"
           -----------------------------------------------
           #"blk" "G" srt
       ];
-  [:| "G" : #"env", "G'" : #"env", "g" : #"sub" %"G" %"G'",
-      "e" : #"blk" %"G'"
+  [:| "G" : #"env", "G'" : #"env", "g" : #"sub" "G" "G'",
+      "e" : #"blk" "G'"
        -----------------------------------------------
-       #"blk_subst" "g" "e" : #"blk" %"G"
+       #"blk_subst" "g" "e" : #"blk" "G"
   ];
-  [:> "G" : #"env", "e" : #"blk" %"G"
+  [:= "G" : #"env", "e" : #"blk" "G"
        ----------------------------------------------- ("blk_subst_id")
-       #"blk_subst" #"id" %"e" = %"e" : #"blk" %"G"
+       #"blk_subst" #"id" "e" = "e" : #"blk" "G"
   ]; 
-  [:> "G1" : #"env", "G2" : #"env", "G3" : #"env",
-       "f" : #"sub" %"G1" %"G2", "g" : #"sub" %"G2" %"G3",
-       "e" : #"blk" %"G3"
+  [:= "G1" : #"env", "G2" : #"env", "G3" : #"env",
+       "f" : #"sub" "G1" "G2", "g" : #"sub" "G2" "G3",
+       "e" : #"blk" "G3"
        ----------------------------------------------- ("blk_subst_cmp")
-       #"blk_subst" %"f" (#"blk_subst" %"g" %"e")
-       = #"blk_subst" (#"cmp" %"f" %"g") %"e"
-       : #"blk" %"G1"
+       #"blk_subst" "f" (#"blk_subst" "g" "e")
+       = #"blk_subst" (#"cmp" "f" "g") "e"
+       : #"blk" "G1"
   ]
   (*TODO: any reason to add halt?
-  [:| "G" : #"env", "v" : #"val" %"G" %"A"
+  [:| "G" : #"env", "v" : #"val" "G" "A"
        -----------------------------------------------
-       #"ret" "v" : #"blk" %"G" %"A"
+       #"ret" "v" : #"blk" "G" "A"
   ];
    
-  [:> "G1" : #"env", "G2" : #"env",
-       "g" : #"sub" %"G1" %"G2",
-       "A" : #"ty", "v" : #"val" %"G2" %"A"
+  [:= "G1" : #"env", "G2" : #"env",
+       "g" : #"sub" "G1" "G2",
+       "A" : #"ty", "v" : #"val" "G2" "A"
        ----------------------------------------------- ("blk_subst_ret")
-       #"blk_subst" %"g" (#"ret" %"v")
-       = #"ret" (#"val_subst" %"g" %"v")
-       : #"blk" %"G1" %"A"
+       #"blk_subst" "g" (#"ret" "v")
+       = #"ret" (#"val_subst" "g" "v")
+       : #"blk" "G1" "A"
   ]*)
-  ]].
+  ]}.
 
 Derive block_subst
        SuchThat (Pre.elab_lang value_subst block_subst_def block_subst)
@@ -61,54 +61,54 @@ Proof. auto_elab. Qed.
 
 
 Definition cps_lang_def : lang :=
-  [[l
+  {[l
       [:| "A" : #"ty"
           -----------------------------------------------
           #"neg" "A" : #"ty"
       ];
   [:| "G" : #"env",
       "A" : #"ty",
-      "e" : #"blk" (#"ext" %"G" %"A")
+      "e" : #"blk" (#"ext" "G" "A")
       -----------------------------------------------
-      #"cont" "A" "e" : #"val" %"G" (#"neg" %"A")
+      #"cont" "A" "e" : #"val" "G" (#"neg" "A")
    ];
    [:| "G" : #"env",
        "A" : #"ty",
-       "v1" : #"val" %"G" (#"neg" %"A"),
-       "v2" : #"val" %"G" %"A"
+       "v1" : #"val" "G" (#"neg" "A"),
+       "v2" : #"val" "G" "A"
       -----------------------------------------------
-      #"jmp" "v1" "v2" : #"blk" %"G"
+      #"jmp" "v1" "v2" : #"blk" "G"
    ];
-  [:> "G" : #"env",
+  [:= "G" : #"env",
       "A" : #"ty",
-      "e" : #"blk" (#"ext" %"G" %"A"),
-      "v" : #"val" %"G" %"A"
+      "e" : #"blk" (#"ext" "G" "A"),
+      "v" : #"val" "G" "A"
       ----------------------------------------------- ("jmp_beta")
-      #"jmp" (#"cont" %"A" %"e") %"v"
-      = #"blk_subst" (#"snoc" #"id" %"v") %"e"
-      : #"blk" %"G"
+      #"jmp" (#"cont" "A" "e") "v"
+      = #"blk_subst" (#"snoc" #"id" "v") "e"
+      : #"blk" "G"
   ];
-  [:> "G" : #"env", "A" : #"ty",
-      "v1" : #"val" %"G" (#"neg" %"A"),
-      "v2" : #"val" %"G" %"A",
+  [:= "G" : #"env", "A" : #"ty",
+      "v1" : #"val" "G" (#"neg" "A"),
+      "v2" : #"val" "G" "A",
       "G'" : #"env",
-      "g" : #"sub" %"G'" %"G"
+      "g" : #"sub" "G'" "G"
       ----------------------------------------------- ("jmp_subst")
-      #"blk_subst" %"g" (#"jmp" %"v1" %"v2")
-      = #"jmp" (#"val_subst" %"g" %"v1") (#"val_subst" %"g" %"v2")
-      : #"blk" %"G'"
+      #"blk_subst" "g" (#"jmp" "v1" "v2")
+      = #"jmp" (#"val_subst" "g" "v1") (#"val_subst" "g" "v2")
+      : #"blk" "G'"
   ];  
-  [:> "G" : #"env", "A" : #"ty",
-      "e" : #"blk" (#"ext" %"G" %"A"),
+  [:= "G" : #"env", "A" : #"ty",
+      "e" : #"blk" (#"ext" "G" "A"),
       "G'" : #"env",
-      "g" : #"sub" %"G'" %"G"
+      "g" : #"sub" "G'" "G"
       ----------------------------------------------- ("cont_subst")
-      #"val_subst" %"g" (#"cont" %"A" %"e")
-      = #"cont" %"A" (#"blk_subst"
-                       (#"snoc" (#"cmp" #"wkn" %"g") #"hd") %"e")
-      : #"val" %"G'" (#"neg" %"A")
+      #"val_subst" "g" (#"cont" "A" "e")
+      = #"cont" "A" (#"blk_subst"
+                       (#"snoc" (#"cmp" #"wkn" "g") #"hd") "e")
+      : #"val" "G'" (#"neg" "A")
   ]
-  ]].
+  ]}.
 
 
 Derive cps_lang
@@ -118,7 +118,6 @@ Derive cps_lang
        As cps_lang_wf.
 Proof. auto_elab. Qed.
 #[export] Hint Resolve cps_lang_wf : elab_pfs.
-
 
 
 Fixpoint wkn_n n :=
@@ -149,11 +148,11 @@ Arguments bind_k n e A k/.
 Definition cps_subst_def : compiler :=
   match # from (exp_subst ++ value_subst) with
   | {{s #"exp" "G" "A"}} =>
-    {{s #"blk" (#"ext" %"G" (#"neg" %"A")) }}
+    {{s #"blk" (#"ext" "G" (#"neg" "A")) }}
   | {{e #"exp_subst" "G" "G'" "g" "A" "e" }} =>
-    {{e #"blk_subst" (#"snoc" (#"cmp" #"wkn" %"g") #"hd") %"e" }}
+    {{e #"blk_subst" (#"snoc" (#"cmp" #"wkn" "g") #"hd") "e" }}
   | {{e #"ret" "G" "A" "v"}} =>
-    {{e #"jmp" #"hd" (#"val_subst" #"wkn" %"v")}}
+    {{e #"jmp" #"hd" (#"val_subst" #"wkn" "v")}}
   end.
 
 Derive cps_subst
@@ -165,109 +164,95 @@ Derive cps_subst
                                           cps_subst
                                           (exp_subst ++ value_subst))
        As cps_subst_preserving.
-Proof.
-  (*TODO: make specialized tactic that doesn't need depth*)
-  assert (wf_lang (cps_lang ++ block_subst ++ value_subst))
-    by eauto 8 with auto_elab elab_pfs.
-
-  setup_elab_compiler.
-
-  all: repeat t.
-  all: solve[by_reduction].
-    Unshelve.
-    all: repeat t'; eauto with elab_pfs auto_elab.
-    all: simpl.
-    all: repeat t'; eauto with elab_pfs auto_elab.
-    (*TODO: why isn't everything simplified already?*)
-Qed.
-(*
-  auto_elab_compiler.
-Qed.
-*)
+Proof. auto_elab_compiler. Qed.
 #[export] Hint Resolve cps_subst_preserving : elab_pfs.
 
 (*TODO: separate file*)
 Definition val_prod_lang_def : lang :=
-  [
-  [:> "G" : #"env", "A" : #"ty", "B" : #"ty",
-      "e" : #"val" %"G" (#"prod" %"A" %"B"),
-      "G'" : #"env",
-      "g" : #"sub" %"G'" %"G"
-      ----------------------------------------------- ("proj_2_subst")
-      #"val_subst" %"g" (#".2" %"e")
-      = #".2" (#"val_subst" %"g" %"e")
-      : #"val" %"G'" %"B"
-  ];
-  [:> "G" : #"env", "A" : #"ty", "B" : #"ty",
-      "e" : #"val" %"G" (#"prod" %"A" %"B"),
-      "G'" : #"env",
-      "g" : #"sub" %"G'" %"G"
-      ----------------------------------------------- ("proj_1_subst")
-      #"val_subst" %"g" (#".1" %"e")
-      = #".1" (#"val_subst" %"g" %"e")
-      : #"val" %"G'" %"A"
-  ];
-  [:> "G" : #"env", "A" : #"ty", "B" : #"ty",
-      "e" : #"val" %"G" %"A",
-      "e'" : #"val" %"G" %"B",
-      "G'" : #"env",
-      "g" : #"sub" %"G'" %"G"
-      ----------------------------------------------- ("pair_subst")
-      #"val_subst" %"g" (#"pair" %"e" %"e'")
-      = #"pair" (#"val_subst" %"g" %"e") (#"val_subst" %"g" %"e'")
-      : #"val" %"G'" (#"prod" %"A" %"B")
-  ];
-  [:> "G" : #"env", "A" : #"ty", "B" : #"ty",
-      "v" : #"val" %"G" (#"prod" %"A" %"B")
-      ----------------------------------------------- ("prod_eta")
-      #"pair" (#".1" %"v") (#".2" %"v") = %"v"
-      : #"val" %"G" (#"prod" %"A" %"B")
-  ];
-  [:> "G" : #"env",
-      "A" : #"ty",
-      "B" : #"ty",
-      "v1" : #"val" %"G" %"A",
-      "v2" : #"val" %"G" %"B"
-      ----------------------------------------------- ("project 2")
-      #".2" (#"pair" %"v1" %"v2") = %"v2"
-      : #"val" %"G" %"B"
-  ];
-  [:> "G" : #"env",
-      "A" : #"ty",
-      "B" : #"ty",
-      "v1" : #"val" %"G" %"A",
-      "v2" : #"val" %"G" %"B"
-      ----------------------------------------------- ("project 1")
-      #".1" (#"pair" %"v1" %"v2") = %"v1"
-      : #"val" %"G" %"A"
-  ];
-    [:| "G" : #"env",
-      "A" : #"ty",
-      "B" : #"ty",
-      "e" : #"val" %"G" (#"prod" %"A" %"B")
-      -----------------------------------------------
-      #".2" "e" : #"val" %"G" %"B"
-   ];
-  [:| "G" : #"env",
-      "A" : #"ty",
-      "B" : #"ty",
-      "e" : #"val" %"G" (#"prod" %"A" %"B")
-      -----------------------------------------------
-      #".1" "e" : #"val" %"G" %"A"
-   ];
-  [:| "G" : #"env",
-      "A" : #"ty",
-      "B" : #"ty",
-      "e1" : #"val" %"G" %"A",
-      "e2" : #"val" %"G" %"B"
-      -----------------------------------------------
-      #"pair" "e1" "e2" : #"val" %"G" (#"prod" %"A" %"B")
-   ];
+  {[l
+      
   [:| "A" : #"ty", "B": #"ty"
       -----------------------------------------------
       #"prod" "A" "B" : #"ty"
-  ] ]%arule.
+  ];
+  [:| "G" : #"env",
+      "A" : #"ty",
+      "B" : #"ty",
+      "e1" : #"val" "G" "A",
+      "e2" : #"val" "G" "B"
+      -----------------------------------------------
+      #"pair" "e1" "e2" : #"val" "G" (#"prod" "A" "B")
+   ];
+  [:| "G" : #"env",
+      "A" : #"ty",
+      "B" : #"ty",
+      "e" : #"val" "G" (#"prod" "A" "B")
+      -----------------------------------------------
+      #".1" "e" : #"val" "G" "A"
+  ];
+  [:| "G" : #"env",
+      "A" : #"ty",
+      "B" : #"ty",
+      "e" : #"val" "G" (#"prod" "A" "B")
+      -----------------------------------------------
+      #".2" "e" : #"val" "G" "B"
+  ];
+  [:= "G" : #"env",
+      "A" : #"ty",
+      "B" : #"ty",
+      "v1" : #"val" "G" "A",
+      "v2" : #"val" "G" "B"
+      ----------------------------------------------- ("project 1")
+      #".1" (#"pair" "v1" "v2") = "v1"
+      : #"val" "G" "A"
+  ];
+  [:= "G" : #"env",
+      "A" : #"ty",
+      "B" : #"ty",
+      "v1" : #"val" "G" "A",
+      "v2" : #"val" "G" "B"
+      ----------------------------------------------- ("project 2")
+      #".2" (#"pair" "v1" "v2") = "v2"
+      : #"val" "G" "B"
+  ];
+  [:= "G" : #"env", "A" : #"ty", "B" : #"ty",
+      "v" : #"val" "G" (#"prod" "A" "B")
+      ----------------------------------------------- ("prod_eta")
+      #"pair" (#".1" "v") (#".2" "v") = "v"
+      : #"val" "G" (#"prod" "A" "B")
+  ];
+  [:= "G" : #"env", "A" : #"ty", "B" : #"ty",
+      "e" : #"val" "G" "A",
+      "e'" : #"val" "G" "B",
+      "G'" : #"env",
+      "g" : #"sub" "G'" "G"
+      ----------------------------------------------- ("pair_subst")
+      #"val_subst" "g" (#"pair" "e" "e'")
+      = #"pair" (#"val_subst" "g" "e") (#"val_subst" "g" "e'")
+      : #"val" "G'" (#"prod" "A" "B")
+  ];
+  [:= "G" : #"env", "A" : #"ty", "B" : #"ty",
+      "e" : #"val" "G" (#"prod" "A" "B"),
+      "G'" : #"env",
+      "g" : #"sub" "G'" "G"
+      ----------------------------------------------- ("proj_1_subst")
+      #"val_subst" "g" (#".1" "e")
+      = #".1" (#"val_subst" "g" "e")
+      : #"val" "G'" "A"
+  ];
+  [:= "G" : #"env", "A" : #"ty", "B" : #"ty",
+      "e" : #"val" "G" (#"prod" "A" "B"),
+      "G'" : #"env",
+      "g" : #"sub" "G'" "G"
+      ----------------------------------------------- ("proj_2_subst")
+      #"val_subst" "g" (#".2" "e")
+      = #".2" (#"val_subst" "g" "e")
+      : #"val" "G'" "B"
+  ]
+  ]}.
 
+
+    
 Derive val_prod_lang
        SuchThat (Pre.elab_lang value_subst val_prod_lang_def val_prod_lang)
        As val_prod_wf.
@@ -278,21 +263,21 @@ Proof. auto_elab. Qed.
 Definition cps_def : compiler :=
   match # from (stlc) with
   | {{s #"exp" "G" "A"}} =>
-    {{s #"blk" (#"ext" %"G" (#"neg" %"A")) }}
+    {{s #"blk" (#"ext" "G" (#"neg" "A")) }}
   | {{e #"->" "A" "B"}} =>
-    {{e #"neg" (#"prod" %"A" (#"neg" %"B")) }}
+    {{e #"neg" (#"prod" "A" (#"neg" "B")) }}
   | {{e #"lambda" "G" "A" "B" "e"}} =>
     (*TODO: use value product or exp-projection product?*)
-    {{e #"cont" (#"prod" %"A" (#"neg" %"B"))
-        (#"blk_subst" (#"snoc" (#"snoc" #"wkn" (#".1" #"hd")) (#".2" #"hd")) %"e") }}
+    {{e #"cont" (#"prod" "A" (#"neg" "B"))
+        (#"blk_subst" (#"snoc" (#"snoc" #"wkn" (#".1" #"hd")) (#".2" #"hd")) "e") }}
   | {{e #"app" "G" "A" "B" "e" "e'"}} =>
-    bind_k 1 (var "e") {{e #"neg" (#"prod" %"A" (#"neg" %"B"))}}
+    bind_k 1 (var "e") {{e #"neg" (#"prod" "A" (#"neg" "B"))}}
     (bind_k 2 (var "e'") (var "A")
     {{e #"jmp" {ovar 1} (#"pair" {ovar 0} {ovar 2}) }})
   | {{e #"exp_subst" "G" "G'" "g" "A" "e" }} =>
-    {{e #"blk_subst" (#"snoc" (#"cmp" #"wkn" %"g") #"hd") %"e" }}
+    {{e #"blk_subst" (#"snoc" (#"cmp" #"wkn" "g") #"hd") "e" }}
   | {{e #"ret" "G" "A" "v"}} =>
-    {{e #"jmp" #"hd" (#"val_subst" #"wkn" %"v")}}
+    {{e #"jmp" #"hd" (#"val_subst" #"wkn" "v")}}
   end.
 
 Derive cps
@@ -305,21 +290,5 @@ Derive cps
                                           cps
                                           stlc)
        As cps_preserving.
-Proof.
-  (*TODO: make specialized tactic that doesn't need depth*)
-  assert (wf_lang (val_prod_lang ++ cps_lang ++ block_subst ++ value_subst))
-    by eauto 8 with auto_elab elab_pfs.
-
-  setup_elab_compiler; repeat t.
-  solve [by_reduction].
-  solve [by_reduction].
-  solve [by_reduction].
-  Unshelve.
-  all: repeat t'; eauto with elab_pfs auto_elab.
-  all: simpl.
-  all: repeat t'; eauto with elab_pfs auto_elab.
-(*
-  auto_elab_compiler.
-*)
-Qed.
+Proof. auto_elab_compiler. Qed.
 #[export] Hint Resolve cps_preserving : elab_pfs.
